txn-data-consistency/EP+_Commutes.thy
@@ -1,0 +1,823 @@
+section \<open>Event commutes for EP+\<close>
+
+theory "EP+_Commutes"
+  imports "EP+" Reductions
+begin
+
+
+subsection \<open>Auxiliary lemmas\<close>
+
+text \<open>Some congruence lemmas for explorative proofs\<close>
+
+lemma fun_upd1_cong: 
+  "\<lbrakk> a = b \<rbrakk> \<Longrightarrow> f(x := a) = f(x := b)"
+  by auto
+
+lemma fun_upd2_cong: 
+  "\<lbrakk> a = c; b = d \<rbrakk> \<Longrightarrow> f(x := a, y := b) = f(x := c, y := d)"
+  by auto
+
+lemma insort_key_arg_cong: "f = g \<Longrightarrow> insort_key f t l = insort_key g t l"
+  by simp
+
+lemma global_conf_rtxn_cls_twisted_update_cong:
+  "s\<lparr>rtxn_rts := b, cls := a\<rparr> = s\<lparr> cls := a, rtxn_rts := b\<rparr>"
+  by auto
+
+thm cl_conf.unfold_congs
+thm global_conf.unfold_congs
+
+lemma global_conf_svrs_cls_twisted_update_cong:
+  "\<lbrakk> X = X'; Y = Y'; Z = Z' \<rbrakk> \<Longrightarrow> s\<lparr>svrs := X, cls := Y, rtxn_rts := Z\<rparr> = s\<lparr>cls := Y', rtxn_rts := Z', svrs := X'\<rparr>" 
+  by auto
+
+lemma global_conf_wtxn_cts_cls_twisted_update_cong:
+  "\<lbrakk> X = X'; Y = Y'; Z = Z' \<rbrakk> \<Longrightarrow> s\<lparr>wtxn_cts := X, cts_order := Y, cls := Z\<rparr> = s\<lparr>cls := Z', wtxn_cts := X', cts_order := Y'\<rparr>"
+  by auto
+
+lemma global_conf_wtxn_cts_cls_rtxn_twisted_update_cong:
+  "\<lbrakk> V = V'; X = X'; Y = Y'; Z = Z' \<rbrakk> \<Longrightarrow>
+    s\<lparr>wtxn_cts := V, cts_order := X, cls := Y, rtxn_rts := Z\<rparr> =
+    s\<lparr>rtxn_rts := Z', cls := Y', wtxn_cts := V', cts_order := X'\<rparr>"
+  by auto
+
+
+(***********************)
+
+lemma wtxns_dom_add_to_readerset [simp]:
+  "wtxns_dom (add_to_readerset (svr_state (svrs s k')) t rts rlst t_wr) 
+ = wtxns_dom (svr_state (svrs s k'))"
+  by (auto simp add: wtxns_dom_def add_to_readerset_def split: ver_state.split)
+
+lemma add_to_readerset_no_ver_inv:
+  "add_to_readerset wtxns t rts rlst t' t'' = No_Ver \<longleftrightarrow> wtxns t'' = No_Ver"
+  by (simp add: add_to_readerset_def split: ver_state.split)
+
+lemma add_to_readerset_prep_inv:
+  "add_to_readerset wtxns t rts rlst t' t'' = Prep ts v \<longleftrightarrow> wtxns t'' = Prep ts v"
+  by (simp add: add_to_readerset_def split: ver_state.split)
+
+lemma add_to_readerset_commit:
+  "add_to_readerset wtxns t rts rlst t' t'' = Commit cts sts lst v rs \<Longrightarrow>
+    \<exists>rs'. wtxns t'' = Commit cts sts lst v rs'"
+  apply (simp add: add_to_readerset_def)
+  by (cases "wtxns t'"; cases "t'' = t'"; auto)
+
+lemma add_to_readerset_pres_get_ts:
+  "get_ts (add_to_readerset wtxns t rts rlst t_wr t') = get_ts (wtxns t')"
+  by (smt (verit, ccfv_SIG) add_to_readerset_commit add_to_readerset_no_ver_inv
+      add_to_readerset_prep_inv ver_state.exhaust_sel ver_state.sel(2))
+
+lemma add_to_readerset_pres_is_committed:
+  "is_committed (add_to_readerset wtxns t rts rlst t_wr t') = is_committed (wtxns t')"
+  by (smt (verit, best) add_to_readerset_no_ver_inv add_to_readerset_prep_inv is_committed.elims(1))
+
+lemma add_to_readerset_pres_at:
+  "at (add_to_readerset wtxns t rts rlst t_wr) ts = at wtxns ts"
+  by (simp add: at_def ver_committed_before_def add_to_readerset_pres_get_ts o_def
+      add_to_readerset_pres_is_committed)
+
+lemma add_to_readerset_pres_newest_own_write:
+  "newest_own_write (add_to_readerset wtxns t rts rlst t_wr) ts cl = newest_own_write wtxns ts cl"
+  by (auto simp add: newest_own_write_def ver_committed_after_def add_to_readerset_pres_get_ts o_def
+      add_to_readerset_pres_is_committed)
+
+lemma add_to_readerset_pres_read_at:
+  "read_at (add_to_readerset wtxns t rts rlst t_wr) ts cl = read_at wtxns ts cl"
+  by (simp add: read_at_def add_to_readerset_pres_at add_to_readerset_pres_get_ts
+      add_to_readerset_pres_newest_own_write)
+
+
+text \<open>View update lemmas\<close>
+
+lemma get_view_update_cls:
+  "cl' \<noteq> cl \<Longrightarrow>
+   get_view (s\<lparr>cls := (cls s)(cl := X) \<rparr>) cl' = get_view s cl'"
+  by (auto simp add: get_view_def)
+
+lemma get_view_update_cls_rtxn_rts:
+  "cl' \<noteq> cl \<Longrightarrow>
+   get_view (s\<lparr>cls := (cls s)(cl := X), rtxn_rts := Y \<rparr>) cl' = get_view s cl'"
+  by (auto simp add: get_view_def)
+
+lemma get_view_update_svr_wtxns_dom:
+   "wtxns_dom new_svr_state = wtxns_dom (svr_state (svrs s k)) \<Longrightarrow> 
+    get_view (s\<lparr>svrs := (svrs s)
+                   (k := svrs s k
+                      \<lparr>svr_state := new_svr_state,
+                       svr_clock := clk \<rparr>)\<rparr>) cl 
+ = get_view s cl"
+  by (auto simp add: get_view_def ext)
+
+
+lemma get_view_update_cls_wtxn_cts_cts_order:
+  "\<lbrakk> cl' \<noteq> cl; wtxn_cts s (get_wtxn s cl) = None; Y > gst (cls s cl') \<rbrakk> \<Longrightarrow>
+   get_view (s\<lparr> cls := (cls s)(cl := X),
+                wtxn_cts := (wtxn_cts s) (get_wtxn s cl \<mapsto> Y),
+                cts_order := Z \<rparr>) cl'
+  = get_view s cl'"
+  by (auto simp add: get_view_def)
+
+lemma get_view_update_svr_prep:
+  assumes "cl \<noteq> get_cl_w t"
+    "t \<noteq> T0"
+    "cl_state (cls s (get_cl_w t)) = WtxnPrep kv_map'"
+    "cl_sn (cls s (get_cl_w t)) = get_sn_w t"
+    "Wtxn_Cts_None s"
+  shows "get_view (s\<lparr>svrs := (svrs s)
+                   (k := svrs s k
+                      \<lparr>svr_state := (svr_state (svrs s k))(t := Prep ts v),
+                       svr_clock := clk \<rparr>)\<rparr>) cl 
+       = get_view s cl"
+  using assms
+  apply (auto simp add: get_view_def wtxns_dom_def)
+  apply (intro ext)
+  by auto
+
+lemma get_view_update_svr_commit:
+   "cl \<noteq> get_cl_w t \<Longrightarrow>
+    svr_state (svrs s k) t = Prep ts v \<Longrightarrow>
+    get_view (s\<lparr>svrs := (svrs s)
+                   (k := svrs s k
+                      \<lparr>svr_state := (svr_state (svrs s k))(t := Commit cts sts lst v rs),
+                       svr_clock := clk,
+                       svr_lst := sclk \<rparr>)\<rparr>) cl
+ = get_view s cl"
+  apply (auto simp add: get_view_def wtxns_dom_def)
+  apply (intro ext)
+  by auto
+
+
+lemmas get_view_update_lemmas = 
+  get_view_update_cls get_view_update_cls_rtxn_rts get_view_update_cls_wtxn_cts_cts_order
+  get_view_update_svr_wtxns_dom get_view_update_svr_prep get_view_update_svr_commit
+
+
+(***********************)
+
+subsection \<open>Commutativity proofs\<close>
+
+\<comment> \<open>read_invoke\<close>
+lemma read_invoke_read_invoke_indep:
+  "cl \<noteq> cl' \<Longrightarrow> left_commute tps (RInvoke cl keys sn) (RInvoke cl' keys' sn')"
+  by (auto simp add: left_commute_def tps_trans_defs fun_upd_twist)
+
+lemma read_invoke_read_indep:
+  "cl \<noteq> cl' \<Longrightarrow> left_commute tps (RInvoke cl keys sn) (Read cl' k' v' t' rts' rlst' sn')"
+  by (auto simp add: left_commute_def tps_trans_defs fun_upd_twist)
+
+lemma read_invoke_read_done_indep:
+  "cl \<noteq> cl' \<Longrightarrow> left_commute tps (RInvoke cl keys sn) (RDone cl' kv_map' sn' u''')"
+  by (auto simp add: left_commute_def tps_trans_defs fun_upd_twist)
+
+lemma read_invoke_write_invoke_indep:
+  "cl \<noteq> cl' \<Longrightarrow> left_commute tps (RInvoke cl keys sn) (WInvoke cl' kv_map' sn')"
+  by (auto simp add: left_commute_def tps_trans_defs fun_upd_twist)
+
+lemma read_invoke_write_commit_indep:
+  "cl \<noteq> cl' \<Longrightarrow> left_commute tps (RInvoke cl keys sn) (WCommit cl' kv_map' cts' sn' u''')"
+  by (auto simp add: left_commute_def tps_trans_defs fun_upd_twist)
+
+lemma read_invoke_write_done_indep:
+  "cl \<noteq> cl' \<Longrightarrow> left_commute tps (RInvoke cl keys sn) (WDone cl' kv_map' sn')"
+  by (auto simp add: left_commute_def tps_trans_defs fun_upd_twist ext)
+
+lemma read_invoke_register_read_indep:
+  "left_commute tps (RInvoke cl keys sn) (RegR k' t' i' rts')"
+  by (auto simp add: left_commute_def tps_trans_defs)
+
+lemma read_invoke_prepare_write_indep:
+  "left_commute tps (RInvoke cl keys sn) (PrepW k' t' v')"
+  by (auto simp add: left_commute_def tps_trans_defs)
+
+lemma read_invoke_commit_write_indep:
+  "left_commute tps (RInvoke cl keys sn) (CommitW k' t' v' cts')"
+  by (auto simp add: left_commute_def tps_trans_defs)
+
+
+\<comment> \<open>read\<close>
+
+lemma read_read_invoke_indep:
+  "cl \<noteq> cl' \<Longrightarrow> left_commute tps (Read cl k v t rts rlst sn) (RInvoke cl' keys' sn')"
+  by (auto simp add: left_commute_def tps_trans_defs fun_upd_twist)
+
+lemma read_read_indep:
+  "cl \<noteq> cl' \<Longrightarrow> left_commute tps (Read cl k v t rts rlst sn) (Read cl' k' v' t' rts' rlst' sn')"
+  by (auto simp add: left_commute_def tps_trans_defs fun_upd_twist)
+
+lemma read_read_done_indep:
+  "cl \<noteq> cl' \<Longrightarrow> left_commute tps (Read cl k v t rts rlst sn) (RDone cl' kv_map' sn' u''')"
+  by (auto simp add: left_commute_def tps_trans_defs fun_upd_twist)
+
+lemma read_write_invoke_indep:
+  "cl \<noteq> cl' \<Longrightarrow> left_commute tps (Read cl k v t rts rlst sn) (WInvoke cl' kv_map' sn')"
+  by (auto simp add: left_commute_def tps_trans_defs fun_upd_twist)
+
+lemma read_write_commit_indep:
+  "cl \<noteq> cl' \<Longrightarrow> left_commute tps (Read cl k v t rts rlst sn) (WCommit cl' kv_map' cts' sn' u''')"
+  by (auto simp add: left_commute_def tps_trans_defs fun_upd_twist)
+
+lemma read_write_done_indep:
+  "cl \<noteq> cl' \<Longrightarrow> left_commute tps (Read cl k v t rts rlst sn) (WDone cl' kv_map' sn')"
+  by (auto simp add: left_commute_def tps_trans_defs fun_upd_twist ext)
+
+lemma read_register_read_indep:
+  "cl \<noteq> get_cl t' \<Longrightarrow> left_commute tps (Read cl k v t_wr rts rlst sn) (RegR k' t' t_wr' rts')"
+  by (auto simp add: left_commute_def tps_trans_defs add_to_readerset_def split: ver_state.split)
+
+lemma read_prepare_write_indep:
+  "left_commute tps (Read cl k v t rts rlst sn) (PrepW k' t' v')"
+  by (auto simp add: left_commute_def tps_trans_defs)
+
+lemma read_commit_write_indep:
+  "left_commute tps (Read cl k v t rts rlst sn) (CommitW k' t' v' cts')"
+  by (auto simp add: left_commute_def tps_trans_defs)
+
+
+\<comment> \<open>read_done\<close>
+
+lemma read_done_read_invoke_indep:
+  "cl \<noteq> cl' \<Longrightarrow> left_commute tps (RDone cl kv_map sn u'') (RInvoke cl' keys' sn')"
+  by (auto simp add: left_commute_def tps_trans_defs fun_upd_twist)
+
+lemma read_done_read_indep:
+  "cl \<noteq> cl' \<Longrightarrow> left_commute tps (RDone cl kv_map sn u'') (Read cl' k' v' t' rts' rlst' sn')"
+  by (auto simp add: left_commute_def tps_trans_defs fun_upd_twist)
+
+lemma read_done_read_done_indep:
+  "cl \<noteq> cl' \<Longrightarrow> left_commute tps (RDone cl kv_map sn u'') (RDone cl' kv_map' sn' u''')"
+  by (auto simp add: left_commute_def tps_trans_defs fun_upd_twist)
+
+lemma read_done_write_invoke_indep:
+  "cl \<noteq> cl' \<Longrightarrow> left_commute tps (RDone cl kv_map sn u'') (WInvoke cl' kv_map' sn')"
+  by (auto simp add: left_commute_def tps_trans_defs fun_upd_twist)
+
+lemma read_done_write_commit_indep:
+  "cl \<noteq> cl' \<Longrightarrow> left_commute tps (RDone cl kv_map sn u'') (WCommit cl' kv_map' cts' sn' u''')"
+  by (auto simp add: left_commute_def tps_trans_defs fun_upd_twist)
+
+lemma read_done_write_done_indep:
+  "cl \<noteq> cl' \<Longrightarrow> left_commute tps (RDone cl kv_map sn u'') (WDone cl' kv_map' sn')"
+  apply (auto simp add: left_commute_def tps_trans_defs fun_upd_twist global_conf_rtxn_cls_twisted_update_cong)
+  apply (intro global_conf.unfold_congs, simp_all)
+  by (intro fun_upd2_cong cl_conf.fold_congs, auto)
+
+lemma read_done_register_read_indep:
+  "left_commute tps (RDone cl kv_map sn u'') (RegR k' t' t_wr' rts')"
+  by (auto simp add: left_commute_def tps_trans_defs)
+
+lemma read_done_prepare_write_indep:
+  "left_commute tps (RDone cl kv_map sn u'') (PrepW k' t' v')"
+  by (auto simp add: left_commute_def tps_trans_defs)
+
+lemma read_done_commit_write_indep:
+  "left_commute tps (RDone cl kv_map sn u'') (CommitW k' t' v' cts')"
+  by (auto simp add: left_commute_def tps_trans_defs)
+
+
+\<comment> \<open>write_invoke\<close>
+
+lemma write_invoke_read_invoke_indep:
+  "cl \<noteq> cl' \<Longrightarrow> left_commute tps (WInvoke cl kv_map sn) (RInvoke cl' keys' sn')"
+  by (auto simp add: left_commute_def tps_trans_defs fun_upd_twist)
+
+lemma write_invoke_read_indep:
+  "cl \<noteq> cl' \<Longrightarrow> left_commute tps (WInvoke cl kv_map sn) (Read cl' k' v' t' rts' rlst' sn')"
+  by (auto simp add: left_commute_def tps_trans_defs fun_upd_twist)
+
+lemma write_invoke_read_done_indep:
+  "cl \<noteq> cl' \<Longrightarrow> left_commute tps (WInvoke cl kv_map sn) (RDone cl' kv_map' sn' u''')"
+  by (auto simp add: left_commute_def tps_trans_defs fun_upd_twist)
+
+lemma write_invoke_write_invoke_indep:
+  "cl \<noteq> cl' \<Longrightarrow> left_commute tps (WInvoke cl kv_map sn) (WInvoke cl' kv_map' sn')"
+  by (auto simp add: left_commute_def tps_trans_defs fun_upd_twist)
+
+lemma write_invoke_write_commit_indep:
+  "cl \<noteq> cl' \<Longrightarrow> left_commute tps (WInvoke cl kv_map sn) (WCommit cl' kv_map' cts' sn' u''')"
+  by (auto simp add: left_commute_def tps_trans_defs fun_upd_twist)
+  
+
+lemma write_invoke_write_done_indep:
+  "cl \<noteq> cl' \<Longrightarrow> left_commute tps (WInvoke cl kv_map sn) (WDone cl' kv_map' sn')"
+  by (auto simp add: left_commute_def tps_trans_defs ext)
+
+lemma write_invoke_register_read_indep:
+  "left_commute tps (WInvoke cl kv_map sn) (RegR k' t' t_wr' rts')"
+  by (auto simp add: left_commute_def tps_trans_defs)
+
+lemma write_invoke_prepare_write_indep:
+  "left_commute tps (WInvoke cl kv_map sn) (PrepW k' t' v')"
+  by (auto simp add: left_commute_def tps_trans_defs)
+
+lemma write_invoke_commit_write_indep:
+  "left_commute tps (WInvoke cl kv_map sn) (CommitW k' t' v' cts')"
+  by (auto simp add: left_commute_def tps_trans_defs)
+
+
+\<comment> \<open>write_commit\<close>
+
+lemma write_commit_read_invoke_indep:
+  "cl \<noteq> cl' \<Longrightarrow> left_commute tps (WCommit cl kv_map cts sn u'') (RInvoke cl' keys' sn')"
+  by (auto simp add: left_commute_def tps_trans_defs fun_upd_twist)
+
+lemma write_commit_read_indep:
+  "cl \<noteq> cl' \<Longrightarrow> left_commute tps (WCommit cl kv_map cts sn u'') (Read cl' k' v' t' rts' rlst' sn')"
+  by (auto simp add: left_commute_def tps_trans_defs fun_upd_twist)
+
+lemma write_commit_read_done_indep:
+  "cl \<noteq> cl' \<Longrightarrow> left_commute tps (WCommit cl kv_map cts sn u'') (RDone cl' kv_map' sn' u''')"
+  by (auto simp add: left_commute_def tps_trans_defs fun_upd_twist)
+
+lemma write_commit_write_invoke_indep:
+  "cl \<noteq> cl' \<Longrightarrow> left_commute tps (WCommit cl kv_map cts sn u'') (WInvoke cl' kv_map' sn')"
+  by (auto simp add: left_commute_def tps_trans_defs fun_upd_twist)
+
+lemma insort_key_same_f:
+  "\<forall>t. t \<noteq> new_t \<longrightarrow> f' t = f t \<Longrightarrow> new_t \<notin> set corder \<Longrightarrow> t \<noteq> new_t \<Longrightarrow>
+    insort_key f' t corder = insort_key f t corder"
+  by (induction corder, auto)
+
+lemma insort_key_comm':
+  "t1 \<notin> set corder \<Longrightarrow> t1 \<noteq> t2 \<Longrightarrow> f t2 \<noteq> X \<Longrightarrow>
+   insort_key (f (t1 := X)) t1 (insort_key f t2 corder) =
+   insort_key (f (t1 := X)) t2 (insort_key (f (t1 := X)) t1 corder)"
+  apply (induction corder, auto)
+  by (metis fun_upd_def insort_key_left_comm remove1_insort_key)+
+
+lemma timestamp_update:
+  "t1 \<noteq> t2 \<Longrightarrow>
+   (\<lambda>t. (the (if t = t2 then Some Y else wtxn_cts s t), Z t))(t1 := (X, Z t1)) =
+   (\<lambda>t. (the (if t = t2 then Some Y else (wtxn_cts s(t1 \<mapsto> X)) t), Z t))"
+  by auto
+
+lemma insort_key_twist:
+  "t1 \<noteq> t2 \<Longrightarrow> t1 \<notin> set corder \<Longrightarrow> t2 \<notin> set corder \<Longrightarrow> (Y, Z t2) \<noteq> (X, Z t1) \<Longrightarrow>
+    insort_key (\<lambda>t. (the (if t = t2 then Some Y else (wtxn_cts s(t1 \<mapsto> X)) t), Z t)) t1
+      (insort_key (\<lambda>t. (the (if t = t2 then Some Y else wtxn_cts s t), Z t)) t2 corder) =
+    insort_key (\<lambda>t. (the (if t = t2 then Some Y else (wtxn_cts s(t1 \<mapsto> X)) t), Z t)) t2
+      (insort_key (\<lambda>t. (the (if t = t1 then Some X else wtxn_cts s t), Z t)) t1 corder)"
+  using insort_key_comm'[of t1 corder t2 "\<lambda>t. (the (if t = t2 then Some Y else wtxn_cts s t), Z t)"
+      "(X, Z t1)"]
+  apply (auto simp add: timestamp_update)
+  apply (intro arg_cong[where f="insort_key _ t2"])
+  by (smt (verit, ccfv_SIG) fun_upd_other insort_key_same_f map_upd_Some_unfold)+
+
+lemma ext_corder_twist:
+  "t1 \<noteq> t2 \<Longrightarrow> \<forall>k. t1 \<notin> set (corder k) \<Longrightarrow> \<forall>k. t2 \<notin> set (corder k) \<Longrightarrow> (Y, Z t2) \<noteq> (X, Z t1) \<Longrightarrow>
+   ext_corder t1 kv_map (\<lambda>t. (the (if t = t2 then Some Y else (wtxn_cts s(t1 \<mapsto> X)) t), Z t))
+     (ext_corder t2 kv_map'
+       (\<lambda>t. (the (if t = t2 then Some Y else wtxn_cts s t), Z t)) corder) =
+   ext_corder t2 kv_map' (\<lambda>t. (the (if t = t2 then Some Y else (wtxn_cts s(t1 \<mapsto> X)) t), Z t))
+     (ext_corder t1 kv_map
+       (\<lambda>t. (the (if t = t1 then Some X else wtxn_cts s t), Z t)) corder)"
+  apply (simp add: ext_corder_def)
+  apply (rule ext, simp, rule conjI)
+   apply (smt (verit, ccfv_SIG) fun_upd_other insort_key_same_f)
+  apply (rule impI, rule conjI)
+   apply (smt (verit, best) fun_upd_other fun_upd_same insort_key_same_f)
+  apply (rule impI, rule conjI)
+   apply (metis option.distinct(1))
+  apply (rule conjI, rule impI)
+   apply (metis option.distinct(1))
+  using insort_key_twist by blast
+
+lemma write_commit_write_commit_indep:    
+  "cl \<noteq> cl' \<Longrightarrow> left_commute tps (WCommit cl kv_map cts sn u'') (WCommit cl' kv_map' cts' sn' u''')"
+  apply (auto simp add: left_commute_def tps_trans_top_defs)
+  subgoal for s by (auto simp add: tps_trans_defs fun_upd_twist)
+  subgoal for s by (auto simp add: tps_trans_defs fun_upd_twist)
+  apply (auto simp add: tps_trans_defs fun_upd_twist)
+  apply (intro global_conf.unfold_congs, simp_all add: unique_ts_def)
+  subgoal for s
+    using ext_corder_twist[of "get_wtxn s cl" "get_wtxn s cl'" "cts_order s"
+       "Max {get_ts (svr_state (svrs s k) (get_wtxn s cl')) |k. k \<in> dom kv_map'}"
+       "\<lambda>t. if t = T0 then 0 else Suc (get_cl_w t)"
+       "Max {get_ts (svr_state (svrs s k) (get_wtxn s cl)) |k. k \<in> dom kv_map}"
+       kv_map s kv_map'] CO_Tid_def[of s cl] CO_Tid_def[of s cl']
+    by (smt (verit) Suc_inject get_cl_w.simps(2) less_irrefl_nat old.prod.inject reach_co_tid
+        txid.distinct(1) txn_state.simps(18))
+  done
+
+lemma write_commit_write_done_indep:
+  "cl \<noteq> cl' \<Longrightarrow> left_commute tps (WCommit cl kv_map cts sn u'') (WDone cl' kv_map' sn')"
+  by (auto simp add: left_commute_def tps_trans_defs ext)
+
+lemma write_commit_register_read_indep:
+  "cl \<noteq> get_cl t' \<Longrightarrow> left_commute tps (WCommit cl kv_map cts sn u'') (RegR k' t' t_wr' rts')"
+  apply (auto simp add: left_commute_def tps_trans_top_defs)
+  apply (auto simp add: tps_trans_GU_defs)
+  subgoal
+    by (smt (verit, ccfv_SIG) add_to_readerset_prep_inv domI option.sel svr_conf.select_convs(1) 
+            svr_conf.surjective svr_conf.update_convs(1) svr_conf.update_convs(2))
+  subgoal
+    by (metis add_to_readerset_pres_get_ts) 
+  done
+
+lemma write_commit_prepare_write_indep:
+  "cl \<noteq> get_cl t' \<Longrightarrow> left_commute tps (WCommit cl kv_map cts sn u'') (PrepW k' t' v')"
+  apply (auto simp add: left_commute_def tps_trans_top_defs)
+  apply (auto simp add: tps_trans_GU_defs)
+  subgoal
+    by (smt (verit, ccfv_SIG) domI fun_upd_other option.sel svr_conf.select_convs(1)
+          svr_conf.surjective svr_conf.update_convs(1) svr_conf.update_convs(2) txid.inject)
+  subgoal 
+    by metis
+  done
+
+lemma write_commit_commit_write_indep:   
+  "cl \<noteq> get_cl t' \<Longrightarrow> left_commute tps (WCommit cl kv_map cts sn u'') (CommitW k' t' v' cts')"
+  apply (auto simp add: left_commute_def tps_trans_top_defs)
+  subgoal for s
+    apply (auto simp add: tps_trans_GU_defs)
+    subgoal 
+      by (smt (verit, ccfv_SIG) domI fun_upd_other option.sel svr_conf.select_convs(1) 
+              svr_conf.simps(7) svr_conf.surjective svr_conf.update_convs(1-2) txid.inject) 
+    subgoal
+      by metis
+    done
+
+  subgoal for s
+    by (auto simp add: tps_trans_GU_defs)
+
+  subgoal for s
+    by (simp add: write_commit_U_def commit_write_U_def)
+
+  done
+
+\<comment> \<open>write_done\<close>
+
+lemma write_done_read_invoke_indep:
+  "cl \<noteq> cl' \<Longrightarrow> left_commute tps (WDone cl kv_map sn) (RInvoke cl' keys' sn')"
+  by (auto simp add: left_commute_def tps_trans_defs fun_upd_twist ext)
+
+lemma write_done_read_indep:
+  "cl \<noteq> cl' \<Longrightarrow> left_commute tps (WDone cl kv_map sn) (Read cl' k' v' t' rts' rlst' sn')"
+  by (auto simp add: left_commute_def tps_trans_defs fun_upd_twist ext)
+
+lemma write_done_read_done_indep:
+  "cl \<noteq> cl' \<Longrightarrow> left_commute tps (WDone cl kv_map sn) (RDone cl' kv_map' sn' u''')"
+  apply (auto simp add: left_commute_def tps_trans_defs fun_upd_twist global_conf_rtxn_cls_twisted_update_cong)
+  apply (intro global_conf.unfold_congs, simp_all)
+  by (intro fun_upd2_cong cl_conf.fold_congs, auto)
+
+lemma write_done_write_invoke_indep:
+  "cl \<noteq> cl' \<Longrightarrow> left_commute tps (WDone cl kv_map sn) (WInvoke cl' kv_map' sn')"
+  by (auto simp add: left_commute_def tps_trans_defs fun_upd_twist ext)
+
+lemma write_done_write_commit_indep:
+  "cl \<noteq> cl' \<Longrightarrow> left_commute tps (WDone cl kv_map sn) (WCommit cl' kv_map' cts' sn' u''')"
+  apply (auto simp add: left_commute_def tps_trans_defs fun_upd_twist global_conf_wtxn_cts_cls_twisted_update_cong)
+  by (intro global_conf.unfold_congs fun_upd2_cong cl_conf.fold_congs, auto)
+
+lemma write_done_write_done_indep:
+  "cl \<noteq> cl' \<Longrightarrow> left_commute tps (WDone cl kv_map sn) (WDone cl' kv_map' sn')"
+  by (auto simp add: left_commute_def tps_trans_defs fun_upd_twist ext)
+
+lemma write_done_server_ev_indep_L: 
+  "{u.
+      \<exists>k. (k = k' \<longrightarrow> u = get_sclk (svr_state (svrs s k') (get_wtxn s cl)) \<and> 
+                      k' \<in> dom kv_map) \<and>
+          (k \<noteq> k' \<longrightarrow> u = get_sclk (svr_state (svrs s k) (get_wtxn s cl)) \<and> k \<in> dom kv_map)} = 
+   {get_sclk (svr_state (svrs s k) (get_wtxn s cl)) |k. k \<in> dom kv_map}"
+  by (auto)
+
+lemma write_done_register_read_indep_L1:
+  "svr_state (svrs s k') t_wr = Commit cts sclk lst v rs \<Longrightarrow>
+   {u.
+      \<exists>k. (k = k' \<longrightarrow> u = sclk \<and> k' \<in> dom kv_map) \<and>
+          (k \<noteq> k' \<longrightarrow> u = get_sclk (svr_state (svrs s k) t_wr) \<and> k \<in> dom kv_map)} = 
+   {get_sclk (svr_state (svrs s k) t_wr) | k. k \<in> dom kv_map}"
+  apply (auto simp add: domIff)
+  by (metis ver_state.sel(5))
+
+lemma write_done_register_read_indep_L2:
+   "(if kv_map k = None
+     then lst_map (cls (s\<lparr>svrs := Z\<rparr>) cl) k
+     else get_lst (svr_state (svrs (s\<lparr>svrs := (svrs s)(k' := svrs s k'\<lparr>
+                     svr_state := svr_state (svrs s k'),
+                     svr_clock := B\<rparr>)\<rparr>) k)
+                  (get_wtxn (s\<lparr>svrs := (svrs s)(k' := X)\<rparr>) cl))) = 
+    (if kv_map k = None 
+     then lst_map (cls s cl) k 
+     else get_lst (svr_state (svrs s k) (get_wtxn s cl)))"
+  by auto
+
+lemma write_done_register_read_indep_L3:
+   "svr_state (svrs s k') t_wr = Commit cts sts lst v rs
+   \<Longrightarrow>
+    (if kv_map k = None
+     then lst_map (cls (s\<lparr>svrs := Z\<rparr>) cl) k
+     else get_lst (svr_state (svrs (s\<lparr>svrs := (svrs s)(k' := svrs s k'\<lparr>
+                     svr_state := (svr_state (svrs s k')) (t_wr := Commit cts sts lst v (insert Y rs)),
+                     svr_clock := B\<rparr>)\<rparr>) k)
+                  (get_wtxn (s\<lparr>svrs := (svrs s)(k' := X)\<rparr>) cl))) = 
+    (if kv_map k = None 
+     then lst_map (cls s cl) k 
+     else get_lst (svr_state (svrs s k) (get_wtxn s cl)))"
+  by auto
+
+lemmas write_done_register_read_indep_lemmas = 
+  write_done_server_ev_indep_L write_done_register_read_indep_L1
+  write_done_register_read_indep_L2 write_done_register_read_indep_L3
+
+lemma write_done_register_read_indep:
+  "cl \<noteq> get_cl t' \<Longrightarrow> left_commute tps (WDone cl kv_map sn) (RegR k' t' t_wr' rts')"
+  apply (auto simp add: left_commute_def tps_trans_top_defs)
+  subgoal for s
+    apply (auto simp add: tps_trans_GU_defs add_to_readerset_def
+                split: if_split_asm ver_state.split)
+    by (smt  domI fun_upd_other fun_upd_same option.inject ver_state.case_eq_if ver_state.exhaust_sel
+        ver_state.sel(2) ver_state.sel(4) ver_state.simps(10))
+
+  subgoal for s
+    by (auto simp add: tps_trans_GU_defs)
+
+  subgoal for s
+    apply (auto simp add: tps_trans_GU_defs add_to_readerset_def
+        write_done_register_read_indep_lemmas split: if_split_asm ver_state.split)
+    done
+  done
+
+lemma write_done_prepare_write_indep_L2:
+   "get_wtxn s cl \<noteq> t'
+   \<Longrightarrow>
+    (if kv_map k = None
+     then lst_map (cls (s\<lparr>svrs := Z\<rparr>) cl) k
+     else get_lst (svr_state (svrs (s\<lparr>svrs := (svrs s)(k' := svrs s k'\<lparr>
+                     svr_state := (svr_state (svrs s k'))(t' := A),
+                     svr_clock := B\<rparr>)\<rparr>) k)
+                  (get_wtxn (s\<lparr>svrs := (svrs s)(k' := X)\<rparr>) cl))) = 
+    (if kv_map k = None 
+     then lst_map (cls s cl) k 
+     else get_lst (svr_state (svrs s k) (get_wtxn s cl)))"
+  by auto
+
+lemmas write_done_prepare_write_indep_lemmas = 
+  write_done_server_ev_indep_L write_done_prepare_write_indep_L2
+
+lemma write_done_prepare_write_indep:
+  "cl \<noteq> get_cl t' \<Longrightarrow> left_commute tps (WDone cl kv_map sn) (PrepW k' t' v')"
+  apply (auto simp add: left_commute_def tps_trans_top_defs)
+  subgoal for s
+    apply (auto simp add: tps_trans_GU_defs)
+    by (smt (verit, ccfv_SIG) domI fun_upd_apply get_cl_w.simps(2) option.inject svr_conf.select_convs(1) 
+            svr_conf.simps(5) svr_conf.simps(6) svr_conf.simps(7) svr_conf.surjective txid0.collapse)
+
+  subgoal for s
+    by (auto simp add: tps_trans_GU_defs)
+
+  subgoal for s
+    apply (auto simp add: tps_trans_GU_defs write_done_prepare_write_indep_lemmas)
+    done
+  done
+
+lemma write_done_commit_write_indep_L2:
+   "get_wtxn s cl \<noteq> t'
+   \<Longrightarrow>
+    (if kv_map k = None
+     then lst_map (cls (s\<lparr>svrs := Z\<rparr>) cl) k
+     else get_lst (svr_state (svrs (s\<lparr>svrs := (svrs s)(k' := svrs s k'\<lparr>
+                     svr_state := (svr_state (svrs s k'))(t' := A),
+                     svr_clock := B, 
+                     svr_lst := C\<rparr>)\<rparr>) k)
+                  (get_wtxn (s\<lparr>svrs := (svrs s)(k' := X)\<rparr>) cl))) = 
+    (if kv_map k = None 
+     then lst_map (cls s cl) k 
+     else get_lst (svr_state (svrs s k) (get_wtxn s cl)))"
+  by auto
+
+lemmas write_done_commit_write_indep_lemmas = 
+  write_done_server_ev_indep_L write_done_commit_write_indep_L2
+
+lemma write_done_commit_write_indep:  
+  "\<lbrakk> cl \<noteq> get_cl t' \<rbrakk>
+  \<Longrightarrow> left_commute tps (WDone cl kv_map sn) (CommitW k' t' v' cts')"
+  apply (auto simp add: left_commute_def tps_trans_top_defs)
+  subgoal for s
+    apply (auto simp add: tps_trans_GU_defs) 
+    by (smt (verit) domI fun_upd_apply get_cl_w.simps(2) option.sel svr_conf.select_convs(1) 
+        svr_conf.simps(5) svr_conf.simps(6) svr_conf.simps(7) svr_conf.surjective txid0.collapse)
+
+  subgoal for s
+    by (auto simp add: tps_trans_GU_defs)
+
+  subgoal for s
+    by (auto simp add: tps_trans_GU_defs write_done_commit_write_indep_lemmas)  (* SLOW *)
+  done
+
+
+\<comment> \<open>register_read\<close>
+
+lemma register_read_read_invoke_indep:
+  "get_cl t \<noteq> cl' \<Longrightarrow> left_commute tps (RegR k t t_wr rts) (RInvoke cl' keys' sn')"
+  by (auto simp add: left_commute_def tps_trans_defs)
+
+lemma register_read_read_indep:
+  "get_cl t \<noteq> cl' \<Longrightarrow> left_commute tps (RegR k t t_wr rts) (Read cl' k' v' t' rts' rlst' sn')"
+  by (auto simp add: left_commute_def tps_trans_defs add_to_readerset_def split: ver_state.split)
+
+lemma register_read_read_done_indep:
+  "get_cl t \<noteq> cl' \<Longrightarrow> left_commute tps (RegR k t t_wr rts) (RDone cl' kv_map' sn' u''')"
+  apply (auto simp add: left_commute_def tps_trans_top_defs)
+  subgoal for s
+    by (auto simp add: tps_trans_GU_defs)
+
+  subgoal for s
+    by (auto simp add: tps_trans_GU_defs)
+
+  subgoal for s
+    by (auto simp add: tps_trans_GU_defs)
+  done 
+
+lemma register_read_write_invoke_indep:
+  "get_cl t \<noteq> cl' \<Longrightarrow> left_commute tps (RegR k t t_wr rts) (WInvoke cl' kv_map' sn')"
+  by (auto simp add: left_commute_def tps_trans_defs)
+
+lemma register_read_write_commit_indep:
+  "get_cl t \<noteq> cl' \<Longrightarrow> left_commute tps (RegR k t t_wr rts) (WCommit cl' kv_map' cts' sn' u''')"
+  apply (auto simp add: left_commute_def tps_trans_top_defs)
+  subgoal for s
+    by (simp_all add: tps_trans_GU_defs)
+
+  subgoal for s
+    apply (auto simp add: tps_trans_GU_defs)
+
+    subgoal for keys kv_map v
+      by (metis add_to_readerset_prep_inv domIff option.inject option.simps(3))
+
+    subgoal for keys kv_map
+      by (metis add_to_readerset_pres_get_ts)
+    done
+
+  subgoal for s
+    by (simp_all add: tps_trans_GU_defs)
+  done
+
+
+lemma register_read_write_done_indep:
+  "get_cl t \<noteq> cl' \<Longrightarrow> left_commute tps (RegR k t t_wr rts) (WDone cl' kv_map' sn')"
+  apply (auto simp add: left_commute_def tps_trans_top_defs)
+  subgoal for s
+    by (auto simp add: tps_trans_GU_defs)
+
+  subgoal for s
+    apply (auto simp add: tps_trans_GU_defs add_to_readerset_def split: if_split_asm ver_state.split)
+    subgoal by (metis domI ver_state.sel(2))
+    subgoal by (metis domIff option.discI option.sel ver_state.sel(4))
+    done
+
+  subgoal for s
+    by (auto simp add: tps_trans_GU_defs add_to_readerset_def write_done_register_read_indep_lemmas 
+             split: if_split_asm ver_state.split) (* SLOW *)
+  done
+
+lemma register_read_register_read_indep:
+  "k \<noteq> k' \<Longrightarrow> left_commute tps (RegR k t t_wr rts) (RegR k' t' t_wr' rts')"
+  by (auto simp add: left_commute_def tps_trans_defs fun_upd_twist)
+
+lemma register_read_prepare_write_indep:
+  "k \<noteq> k' \<Longrightarrow> left_commute tps (RegR k t t_wr rts) (PrepW k' t' v')"
+  by (auto simp add: left_commute_def tps_trans_defs fun_upd_twist)
+
+lemma register_read_commit_write_indep:
+  "k \<noteq> k' \<Longrightarrow> left_commute tps (RegR k t t_wr rts) (CommitW k' t' v' cts')"
+  by (auto simp add: left_commute_def tps_trans_defs fun_upd_twist)
+
+
+\<comment> \<open>prepare_write\<close>
+
+lemma prepare_write_read_invoke_indep:
+  "get_cl t \<noteq> cl' \<Longrightarrow> left_commute tps (PrepW k t v) (RInvoke cl' keys' sn')"
+  by (auto simp add: left_commute_def tps_trans_defs)
+
+lemma prepare_write_read_indep:
+  "get_cl t \<noteq> cl' \<Longrightarrow> left_commute tps (PrepW k t v) (Read cl' k' v' t' rts' rlst' sn')"
+  by (auto simp add: left_commute_def tps_trans_defs)
+
+lemma prepare_write_read_done_indep:
+  "get_cl t \<noteq> cl' \<Longrightarrow> left_commute tps (PrepW k t v) (RDone cl' kv_map' sn' u''')"
+  apply (auto simp add: left_commute_def read_done_def prepare_write_def)
+  subgoal for s
+    by (auto simp add: tps_trans_GU_defs)
+
+  subgoal for s
+    by (auto simp add: tps_trans_defs)
+
+  subgoal for s
+    by (auto simp add: tps_trans_GU_defs)
+  done 
+
+lemma prepare_write_write_invoke_indep:
+  "get_cl t \<noteq> cl' \<Longrightarrow> left_commute tps (PrepW k t v) (WInvoke cl' kv_map' sn')"
+  by (auto simp add: left_commute_def tps_trans_defs)
+
+lemma prepare_write_write_commit_indep:
+  "get_cl t \<noteq> cl' \<Longrightarrow> left_commute tps (PrepW k t v) (WCommit cl' kv_map' cts' sn' u''')"
+  apply (auto simp add: left_commute_def tps_trans_top_defs)
+  subgoal for s
+    by (auto simp add: tps_trans_GU_defs)
+  
+  subgoal for s
+    apply (auto simp add: tps_trans_GU_defs)
+    by metis
+
+  subgoal for s
+    by (auto simp add: tps_trans_GU_defs)
+  done
+
+lemma prepare_write_write_done_indep:
+  "get_cl t \<noteq> cl' \<Longrightarrow> left_commute tps (PrepW k t v) (WDone cl' kv_map' sn')"
+  apply (auto simp add: left_commute_def prepare_write_def write_done_def)
+  by (auto simp add: write_done_G_def write_done_U_def prepare_write_G_def prepare_write_U_def
+                     write_done_prepare_write_indep_lemmas)
+
+lemma prepare_write_register_read_indep:
+  "k \<noteq> k' \<Longrightarrow> left_commute tps (PrepW k t v) (RegR k' t' t_wr' rts')"
+  by (auto simp add: left_commute_def tps_trans_defs fun_upd_twist)
+
+lemma prepare_write_prepare_write_indep:
+  "k \<noteq> k' \<Longrightarrow> left_commute tps (PrepW k t v) (PrepW k' t' v')"
+  by (auto simp add: left_commute_def tps_trans_defs fun_upd_twist)
+
+lemma prepare_write_commit_write_indep:
+  "k \<noteq> k' \<Longrightarrow> left_commute tps (PrepW k t v) (CommitW k' t' v' cts')"
+  by (auto simp add: left_commute_def tps_trans_defs fun_upd_twist)
+
+\<comment> \<open>commit_write\<close>
+
+lemma commit_write_read_invoke_indep:
+  "get_cl t \<noteq> cl' \<Longrightarrow> left_commute tps (CommitW k t v cts) (RInvoke cl' keys' sn')"
+  by (auto simp add: left_commute_def tps_trans_defs)
+
+lemma commit_write_read_indep:
+  "get_cl t \<noteq> cl' \<Longrightarrow> left_commute tps (CommitW k t v cts) (Read cl' k' v' t' rts' rlst' sn')"
+  by (auto simp add: left_commute_def tps_trans_defs) 
+
+lemma commit_write_read_done_indep:
+  "get_cl t \<noteq> cl' \<Longrightarrow> left_commute tps (CommitW k t v cts) (RDone cl' kv_map' sn' u''')"
+  apply (auto simp add: left_commute_def read_done_def commit_write_def)
+  subgoal for s
+    by (auto simp add: tps_trans_defs)
+
+  subgoal for s
+    by (auto simp add: tps_trans_defs)
+
+  subgoal for s
+    by (auto simp add: tps_trans_defs)
+  done 
+
+lemma commit_write_write_invoke_indep:
+  "get_cl t \<noteq> cl' \<Longrightarrow> left_commute tps (CommitW k t v cts) (WInvoke cl' kv_map' sn')"
+  by (auto simp add: left_commute_def tps_trans_defs)
+
+lemma commit_write_write_commit_indep:
+  "get_cl t \<noteq> cl' \<Longrightarrow> left_commute tps (CommitW k t v cts) (WCommit cl' kv_map' cts' sn' u''')"
+  apply (auto simp add: left_commute_def tps_trans_top_defs) 
+  subgoal for s
+    by (auto simp add: tps_trans_GU_defs)
+
+  subgoal for s
+    apply (auto simp add: tps_trans_GU_defs)
+    by metis+
+
+  subgoal for s
+    by (auto simp add: tps_trans_GU_defs)
+  done
+
+lemma commit_write_write_done_indep:
+  "get_cl t \<noteq> cl' \<Longrightarrow> left_commute tps (CommitW k t v cts) (WDone cl' kv_map' sn')"
+  apply (auto simp add: left_commute_def tps_trans_top_defs)
+  subgoal for s
+    by (auto simp add: tps_trans_GU_defs)
+
+  subgoal for s
+    by (auto simp add: tps_trans_GU_defs)
+
+  subgoal for s 
+    by (auto simp add: tps_trans_GU_defs write_done_commit_write_indep_lemmas)  (* SLOW, ~15s *)
+  done                                                                                                               
+
+lemma commit_write_register_read_indep:
+  "k \<noteq> k' \<Longrightarrow> left_commute tps (CommitW k t v cts) (RegR k' t' t_wr' rts')"
+  by (auto simp add: left_commute_def tps_trans_defs fun_upd_twist)
+
+lemma commit_write_prepare_write_indep:
+  "k \<noteq> k' \<Longrightarrow> left_commute tps (CommitW k t v cts) (PrepW k' t' v')"
+  by (auto simp add: left_commute_def tps_trans_defs fun_upd_twist)
+
+lemma commit_write_commit_write_indep:
+  "k \<noteq> k' \<Longrightarrow> left_commute tps (CommitW k t v cts) (CommitW k' t' v' cts')"
+  by (auto simp add: left_commute_def tps_trans_defs fun_upd_twist)
+
+
+\<comment> \<open>Skip\<close>
+lemma skip_e_indep:
+  "left_commute tps Skip2 e"
+  by (auto simp add: left_commute_def)
+
+lemma e_skip_indep:
+  "left_commute tps e Skip2"
+  by (auto simp add: left_commute_def)
+
+end
